Commit

Compiler/CodeGenM.v
@@ -98,9 +98,9 @@ Definition assnST : Type := nat -> stmt -> GModule -> Prop.
 
 Definition ST_ok {T} (P : assnST) (gen : CUDAM T) (Q : T -> assnST) :=
   forall n n' st st' GM GM' v,
-    P n st GM 
-    -> gen (n, (st, GM)) = (v, (n', (st', GM')))
-    -> Q v n' st' GM'.
+    P n (seqs st) GM 
+    -> gen n GM = (v, (n', st', GM'))
+    -> Q v n' ((seqs (st ++ st'))) GM'.
 
 Definition FC_ok (G : FC) : assnST := fun _ _ gm => sat_FC gm G G.
 Parameter fv_assn : assn -> list var -> Prop.
@@ -181,15 +181,69 @@ Proof.
   intros Hmn H; induction H; constructor; eauto using usable_var_weaken.
 Qed.
 
+Lemma safe_seqs_app : forall GM (n : nat) (C1 C2 : list stmt) (s : stack) (h : zpheap) (P Q : assn),
+   safe_nh GM n s h (seqs C1) P
+   -> (forall s h m, sat s (as_gheap h) P -> m <= n -> safe_nh GM n s h (seqs C2) Q)
+   -> safe_nh GM n s h (seqs (C1 ++ C2)) Q.
+Proof.
+  induction n; [simpl; eauto|].
+  introv.
+  intros (Hskip & Hab1 & Hstep1) Hsafe2; split; [|split].
+  - Lemma seqs_skip C : seqs C = host_skip -> C = nil.
+    Proof.
+      induction C; simpl; try congruence.
+    Qed.
+    intros Hsk; apply seqs_skip, app_eq_nil in Hsk.
+    destruct Hsk; substs; simpl in Hskip.
+    forwards*: Hskip; forwards*: Hsafe2; simpl in *; jauto.
+  - Lemma seqs_app_abort GM C1 C2 s h :
+      aborts_h GM (seqs (C1 ++ C2)) s h
+      -> aborts_h GM (seqs C1) s h \/ (C1 = nil).
+    Proof.
+      induction C1; simpl; eauto.
+      intros Hab; inverts Hab.
+      left; constructor; eauto.
+    Qed.
+    introv Hdis Heq Hab; forwards* [Hab' | ?]: (>>seqs_app_abort Hab); substs.
+    simpl in *; forwards*: Hskip; forwards*: Hsafe2.
+  - introv Hdis Heq Hstep.
+    Lemma seqs_app_step GM C1 C2 C' st1 st2 :
+      stmt_exec GM (seqs (C1 ++ C2)) st1 C' st2
+      -> (exists C'', stmt_exec GM (seqs C1) st1 (seqs C'') st2 /\ seqs (C'' ++ C2) = C')  \/
+         (C1 = nil).
+    Proof.
+      induction C1; simpl; eauto.
+      intros Hstep; inverts Hstep.
+      - left; exists (s1' :: C1); split; constructor; eauto.
+      - left; exists C1; split; eauto; constructor.
+    Qed.
+    forwards*[(C' & Hstep' & ?) | ?]: (>>seqs_app_step Hstep); substs; jauto.
+    + forwards* (h'' & ? & ? & ?): Hstep1; exists h''; splits; jauto.
+      applys* IHn; intros; forwards*: (>>Hsafe2 n).
+      applys (>>safe_nh_mono); eauto.
+    + simpl in Hstep.
+      forwards*: Hskip; forwards* (? & ? & Hsafe2'): Hsafe2.
+Qed.
+
+Lemma rule_app_seqs GM G P Q R st1 st2 :
+  CSLh_n GM G P (seqs st1) Q
+  -> CSLh_n GM G Q (seqs st2) R
+  -> CSLh_n GM G P (seqs (st1 ++ st2)) R.
+Proof.
+  unfold CSLh_n, CSLh_n_simp; intros H1 H2; intros.
+  eauto using safe_seqs_app.
+Qed.
+
 Lemma rule_fresh G P Q xs ys:
   ST_ok (code_ok G P Q xs ys) 
         fresh
         (fun y => code_ok G P Q xs (y :: ys)).
 Proof.
-  unfold ST_ok, fresh, setS, code_ok.
+  unfold ST_ok, fresh, setC, code_ok.
   introv (Hfs & Htri & Hxs & Hys & Henv & Hdisj) Heq.
   inverts Heq.
   splits; eauto.
+  - rewrite app_nil_r; eauto.
   - applys (>>usable_weaken Hxs); omega.
   - constructor.
     + apply lt_usable_var; omega.
@@ -256,6 +310,24 @@ Proof.
   intros [? | ?]; eauto.
 Qed.
 
+Lemma rule_hseq GM G st st' P Q R:
+  CSLh_n GM G P st Q 
+  -> CSLh_n GM G Q st' R
+  -> CSLh_n GM G P (hseq st st') R.
+Proof.
+  intros.
+  destruct st'; simpl; eauto using rule_host_seq.
+  intros n Hfc s h Hp.
+  forwards*: (>>H0 n Hfc).
+  forwards*: (>>H n Hfc s h Hp).
+  clear Hp H; revert s h st H1 H2; clear; induction n; simpl; eauto; introv.
+  intros Htri (? & ? & ?); splits; eauto.
+  - intros; substs; forwards*H': H; forwards*: (>>Htri H); simpl in *; jauto.
+  - intros; forwards*(h'' & ? & ?): H1; exists h''; splits; jauto.
+    applys* IHn.
+    intros ? ? Hq; forwards*: Htri; eauto using safe_nh_mono.
+Qed.
+
 Lemma rule_setI G P Q R ss xs xs' ys :
   (forall GM, CSLh_n GM G Q ss R)
   -> (fv_assn R (xs ++ xs'))
@@ -264,10 +336,11 @@ Lemma rule_setI G P Q R ss xs xs' ys :
            (setI ss)
            (fun _ => code_ok G P R (xs ++ xs') (remove_xs ys xs')).
 Proof.
-  unfold ST_ok, setI, setS, code_ok.
+  unfold code_ok.
   introv Htri Hfv Hxs' (Hfs & Htr & Hxs & Hys & Henv & Hdisj) Heq; simpl in *.
   inverts Heq; splits; jauto.   
-  - eapply rule_host_seq; eauto.
+  - eapply rule_app_seqs; eauto; simpl.
+    eapply rule_host_seq; eauto using rule_host_skip.
   - apply usable_app; eauto.
     applys* usable_incl.
   - eapply usable_incl; [|eauto using remove_xs_incl]; eauto.
@@ -279,18 +352,19 @@ Qed.
 
 Definition nST P : assnST := fun n _ _ => P n.
 
-Instance CUDAM_Monad : Monad CUDAM := state_Monad _.
-
-Lemma rule_bind T1 T2 P (Q Q' : T1 -> assnST) R (gen : CUDAM T1) (gen' : T1 -> CUDAM T2) :
+Lemma rule_bind T1 T2 P (Q : T1 -> assnST) R (gen : CUDAM T1) (gen' : T1 -> CUDAM T2) :
   ST_ok P gen Q
-  -> (forall x n st gm, Q x n st gm -> Q' x n st gm)
-  -> (forall x, ST_ok (Q' x) (gen' x) R)
-  -> ST_ok P (do! x := gen in gen' x) R.
+  -> (forall x, ST_ok (Q x) (gen' x) R)
+  -> ST_ok P (do! x <- gen in gen' x) R.
 Proof.
   unfold ST_ok in *; intros.
-  inverts H3.
-  destruct (gen _) as (? & ? & ? & ?) eqn:Heq.
+  inverts H2.
+  destruct (gen _ _) as (? & ((? & ?) & ?)) eqn:Heq.
   forwards*: H.
+  destruct (gen' _ _) as (? & ((? & ?) & ?)) eqn:Heq'.
+  forwards*: H0.
+  inverts H4.
+  rewrite app_assoc; eauto.
 Qed.
 
 Lemma remove_var_incl Env x:
@@ -308,9 +382,11 @@ Lemma rule_ret (T : Set) (v : T) (P : T -> assnST) :
   ST_ok (P v) (ret v : CUDAM T) (fun (x : T) => P x).
 Proof.
   unfold ST_ok; introv ? H'; inverts H'; simpl; eauto.
+  rewrites* app_nil_r.
 Qed.
 
 Arguments ret {f _ A} x : simpl never.
+Arguments bind {f _ A B} _ _ : simpl never.
 Lemma rule_forward T (P' P : assnST) (Q : T -> assnST) gen :
   ST_ok P gen Q -> (forall n c gm, P' n c gm -> P n c gm) -> ST_ok P' gen Q.
 Proof.
@@ -341,9 +417,9 @@ Lemma rule_fLet G Pre R P E xs ys e v :
            (fun x => code_ok G Pre (Assn R P (x |-> v :: E)) (x :: xs) (remove_xs ys (x :: nil))).
 Proof.
   unfold fLet; intros Hveal.
-  eapply rule_bind; [apply rule_fresh|eauto |].
+  eapply rule_bind; [apply rule_fresh| ].
   introv; apply code_ok_float; intros Hincl Hdisj; simpl in Hdisj.
-  eapply rule_bind; [|eauto|].
+  eapply rule_bind.
   { applys* (>>rule_setI (x :: nil)).
     - intros; applys* rule_host_let.
     - rewrite fv_assn_base in *; simpl.
@@ -376,6 +452,12 @@ Proof.
       apply remove_xs_incl.
 Qed.
 
+Definition ex_st {T} (f : T -> assnST) : assnST :=
+  fun n st gm => exists x, f x n st gm.
+
+Notation "'Ex_st' x .. y , p" := (ex_st (fun x => .. (ex_st (fun y => p)) ..))
+  (at level 200, x binder, right associativity).
+
 Lemma rule_fAlloc G Pre R P E xs ys e size :
   evalExp E e (Zn size)
   -> ST_ok (code_ok G Pre (Assn R P E) xs ys)
@@ -385,9 +467,9 @@ Lemma rule_fAlloc G Pre R P E xs ys e size :
                              (x :: xs) (remove_xs ys (x :: nil))).
 Proof.
   unfold fLet; intros Hveal.
-  eapply rule_bind; [apply rule_fresh|eauto |].
+  eapply rule_bind; [apply rule_fresh|].
   introv; apply code_ok_float; intros Hincl Hdisj; simpl in Hdisj.
-  eapply rule_bind; [|eauto|].
+  eapply rule_bind; [|].
   { applys* (>>rule_setI (x :: nil)).
     - intros; applys* rule_host_alloc.
     - repeat (rewrite fv_assn_Ex; introv); rewrite fv_assn_base in *; simpl.
@@ -420,46 +502,49 @@ Proof.
       apply remove_xs_incl.
 Qed.
 
-Lemma rule_fAllocs G Pre R P E xs ys e size :
-  evalExp E e (Zn size)
-  -> ST_ok (code_ok G Pre (Assn R P E) xs ys)
-           (fAlloc e)
-           (fun x => code_ok G Pre (Ex p vs, Assn (array (GLoc p) vs 1 *** R) (length vs = size /\ P)
-                                                  (x |-> p :: E))
-                             (x :: xs) (remove_xs ys (x :: nil))).
+Lemma rule_backward T (P : assnST) (Q Q' : T -> assnST) gen :
+  ST_ok P gen Q -> (forall n c gm x, Q x n c gm -> Q' x n c gm) -> ST_ok P gen Q'.
 Proof.
-  unfold fLet; intros Hveal.
-  eapply rule_bind; [apply rule_fresh|eauto |].
-  introv; apply code_ok_float; intros Hincl Hdisj; simpl in Hdisj.
-  eapply rule_bind; [|eauto|].
-  { applys* (>>rule_setI (x :: nil)).
-    - intros; applys* rule_host_alloc.
-    - repeat (rewrite fv_assn_Ex; introv); rewrite fv_assn_base in *; simpl.
-      unfold incl; simpl.
-      introv; repeat (rewrite in_app_iff; simpl).
-      intros [? | ?]; substs; eauto.
-      left; apply Hincl.
-      forwards*: remove_var_incl'. 
-    - unfold incl; simpl; intros ? [|[]]; eauto. }
-  introv.
-  eapply rule_forward; [apply rule_ret|].
-  introv (Hfs & Htri & Hxs & Hys & Henv' & Hdisj'); splits; eauto.
-  - cutrewrite (E = remove_var E x); [eauto|].
-    rewrites fv_assn_base in Hincl.
-    rewrites* remove_var_disjoint.
-  - applys* (>>usable_incl Hxs).
-    unfold incl; simpl; introv [? | ?]; substs; eauto;
-    repeat (rewrite in_app_iff; simpl); eauto.
-  - applys* (>>usable_incl Hys); unfold incl; introv ?.
-    simpl; destruct var_eq_dec; try congruence.
-  - repeat (rewrite fv_assn_Ex; introv); rewrite fv_assn_base in *; unfold incl in *; simpl.
-    intros ? [?|?]; eauto.
-  - apply disjoint_comm; simpl; split.
-    + intros Hc.
-      forwards*: (disjoint_remove_xs ys (x :: nil)).
-      apply disjoint_comm in H; simpl in H; jauto.
-    + destruct Hdisj as [_ Hdisj].
-      apply disjoint_comm in Hdisj.
-      applys (>>disjoint_incl Hdisj).
-      apply remove_xs_incl.
+  unfold ST_ok; eauto.
+Qed.
+
+Lemma rule_fAllocs typ G Pre R P E xs ys (sz : var) size :
+  evalExp E sz (Zn size)
+  -> ST_ok (code_ok G Pre (Assn R P E) xs ys)
+           (fAllocs' typ sz)
+           (fun ls => code_ok G Pre (Ex ps vs, Assn (arrays (val2gl ps) vs 1 *** R)
+                                                    (length vs = size /\ P)
+                                                    (ls |=> ps ++ E))
+                              (flatTup ls ++ xs) (remove_xs ys (flatTup ls))).
+Proof.
+  revert R P E xs ys; induction typ; simpl; eauto; introv Heval.
+  - eapply rule_backward; [applys* rule_fAlloc |].
+    simpl; introv (? & ? & ? & ? & ? & ?); splits; eauto.
+    + eapply rule_host_backward; eauto.
+      introv (p & vs & Hsat); exists p vs; revert s h Hsat; prove_imp.
+      rewrite mkReduce.arrays_TB; eauto.
+    + rewrite fv_assn_Ex in *; intros ps; specialize (H3 ps).
+      rewrite fv_assn_Ex in *; intros vs; specialize (H3 vs).
+      rewrites* fv_assn_base in *.
+  - eapply rule_backward; [applys* rule_fAlloc |].
+    simpl; introv (? & ? & ? & ? & ? & ?); splits; eauto.
+    + eapply rule_host_backward; eauto.
+      introv (p & vs & Hsat); exists p vs; revert s h Hsat; prove_imp.
+      rewrite mkReduce.arrays_TZ; eauto.
+    + rewrite fv_assn_Ex in *; intros ps; specialize (H3 ps).
+      rewrite fv_assn_Ex in *; intros vs; specialize (H3 vs).
+      rewrites* fv_assn_base in *.
+  - simpl.
+    eapply rule_bind; eauto.
+    introv; simpl.
+    Lemma rule_ex_gen A T G Pre Pst xs ys G' Pre' Pst' xs' ys' (gen : CUDAM A) : 
+      (forall x : T, ST_ok (code_ok G Pre (Pst x) xs ys) gen
+                           (fun x => code_ok (G' x) (Pre' x) (Pst' x) (xs' x) (ys' x)))
+      -> ST_ok (code_ok G Pre (Ex x : T, Pst x) xs ys) gen
+               (fun x => code_ok (G' x) (Pre' x) (Pst' x) (xs' x) (ys' x)).
+    Proof.
+      unfold ST_ok; introv Hsat Hok Hgen.
+      unfold code_ok in *.
+      forwards*: Hsat.
+      splits; jauto.      
 Qed.
